messageInvariantPrototypes/twoPhaseCommit/centralized/system.dfy
@@ -1,0 +1,113 @@
+
+include "hosts.dfy"
+
+module System {
+  import opened UtilitiesLibrary
+  import opened Types
+  import Host
+  import CoordinatorHost
+  import ParticipantHost
+
+  datatype Constants = Constants(hosts: seq<Host.Constants>)
+  {
+    predicate WF() {
+      Host.GroupWFConstants(hosts)
+    }
+    predicate ValidHostId(id: HostId) {
+      id < |hosts|
+    }
+
+    predicate ValidParticipantId(id: HostId) {
+      id < |hosts|-1
+    }
+
+    predicate ValidCoordinatorId(id: HostId) {
+      id == |hosts|-1
+    }
+  }
+
+  datatype Variables = Variables(hosts: seq<Host.Variables>)
+  {
+    predicate WF(c: Constants) {
+      && c.WF()
+      && Host.GroupWF(c.hosts, hosts)
+    }
+  }
+
+  predicate Init(c: Constants, v: Variables)
+  {
+    && v.WF(c)
+    && Host.GroupInit(c.hosts, v.hosts)
+  }
+
+  datatype Step =
+    | VoteReqStep(coordinator: HostId)
+    | SendVoteStep(participant: HostId, coordinator: HostId, vote: Vote)
+    | DecideStep(coordinator: HostId, decision: Decision)
+    | StutterStep()
+
+    
+  predicate NextVoteReqStep(c: Constants, v: Variables, v': Variables, cidx: HostId) 
+    requires v.WF(c) && v'.WF(c)
+  {
+    var cLbl := CoordinatorHost.VoteReqLbl();
+    var pLbl := ParticipantHost.VoteReqLbl();
+    && c.ValidCoordinatorId(cidx)
+    && Host.Next(c.hosts[cidx], v.hosts[cidx], v'.hosts[cidx], Host.CL(cLbl))
+    && (forall pidx:nat | c.ValidParticipantId(pidx)
+        :: Host.Next(c.hosts[pidx], v.hosts[pidx], v'.hosts[pidx], Host.PL(pLbl))
+    )
+  }
+
+  predicate NextSendVoteStep(c: Constants, v: Variables, v': Variables, pidx: HostId, cidx: HostId, vote: Vote) 
+    requires v.WF(c) && v'.WF(c)
+  {
+    var cLbl := CoordinatorHost.ReceiveVoteLbl(vote, pidx);
+    var pLbl := ParticipantHost.SendVoteLbl(vote);
+    && c.ValidCoordinatorId(cidx)
+    && c.ValidParticipantId(pidx)
+    && Host.Next(c.hosts[cidx], v.hosts[cidx], v'.hosts[cidx], Host.CL(cLbl))
+    && Host.Next(c.hosts[pidx], v.hosts[pidx], v'.hosts[pidx], Host.PL(pLbl))
+    && (forall id:nat | c.ValidHostId(id) && id != cidx && id != pidx
+        :: v.hosts[id] == v'.hosts[id]
+    )
+  }
+
+  predicate NextDecideStep(c: Constants, v: Variables, v': Variables, cidx: HostId, decision: Decision)
+    requires v.WF(c) && v'.WF(c)
+  {
+    var cLbl := CoordinatorHost.DecideLbl(decision);
+    var pLbl := ParticipantHost.DecideLbl(decision);
+    && c.ValidCoordinatorId(cidx)
+    && Host.Next(c.hosts[cidx], v.hosts[cidx], v'.hosts[cidx], Host.CL(cLbl))
+    && (forall pidx:nat | c.ValidParticipantId(pidx)
+        :: Host.Next(c.hosts[pidx], v.hosts[pidx], v'.hosts[pidx], Host.PL(pLbl))
+    )
+  }
+
+  predicate NextStep(c: Constants, v: Variables, v': Variables, step: Step)
+    requires v.WF(c) && v'.WF(c)
+  {
+    match step
+      case VoteReqStep(cidx) => NextVoteReqStep(c, v, v', cidx)
+      case SendVoteStep(pidx, cidx, vote) => NextSendVoteStep(c, v, v', pidx, cidx, vote)
+      case DecideStep(cidx, decision) => NextDecideStep(c, v, v', cidx, decision)
+      case StutterStep => && v == v'
+  }
+
+  predicate Next(c: Constants, v: Variables, v': Variables)
+  {
+    && v.WF(c)
+    && v'.WF(c)
+    && exists step :: NextStep(c, v, v', step)
+  }
+
+  function GetDecisionForHost(hv: Host.Variables) : Option<Decision>
+  {
+    match hv
+      case CoordinatorVariables(coordinator) => coordinator.decision
+      case ParticipantVariables(participant) => participant.decision
+  }
+}
+
+
